examples/lowparse/LowParse.Impl.VLBytes.Part2.Subpart1.fst
@@ -1,7 +1,7 @@
 module LowParse.Impl.VLBytes.Part2.Subpart1
 include LowParse.Impl.VLBytes.Part1
 
-#set-options "--z3rlimit 32"
+#set-options "--z3rlimit 1024 --max_fuel 8 --max_ifuel 8"
 
 let parse_bounded_integer'_1_correct
   (b: bytes)
